Add `array_init` and corresponding WP specs.

theories/heap_lang/lib/array.v
@@ -31,6 +31,19 @@ Definition array_clone : val :=
     array_copy_to "dst" "src" "n";;
     "dst".
 
+Definition array_init_loop : val :=
+  rec: "loop" "src" "i" "n" "f" :=
+    if: "i" = "n" then #()
+    else "src" +ₗ "i" <- "f" "i";;
+         "loop" "src" ("i" + #1) "n" "f".
+
+(* similar to [Array.init] in OCaml's stdlib *)
+Definition array_init : val :=
+  λ: "n" "f",
+    let: "src" := AllocN "n" #() in
+    array_init_loop "src" #0 "n" "f";;
+    "src".
+
 Section proof.
   Context `{!heapG Σ}.
 
@@ -105,6 +118,91 @@ Section proof.
   Proof.
     iIntros (? ? Φ) "H HΦ". iApply (twp_wp_step with "HΦ").
     iApply (twp_array_clone with "H"); [auto..|]; iIntros (l') "H HΦ". by iApply "HΦ".
+  Qed.
+
+  (* TODO: move to std++? *)
+  Lemma insert_0_replicate {A : Type} (x y : A) n :
+    <[0:=y]>(replicate (S n) x) = y :: replicate n x.
+  Proof. by induction n; eauto. Qed.
+
+  Lemma wp_array_init_loop {A : Type} (g : A → val) (Q : nat → A → iProp Σ)
+          (xs : list A) i n l (f : val) stk E :
+    (0 < n) →
+    length xs = i →
+    (i ≤ n) →
+    ([∗ list] k↦x∈xs, Q k x) -∗
+    (□ ∀ i : nat, WP f #i @ stk; E {{ v, ∃ x : A, ⌜v = g x⌝ ∗ Q i x }}) -∗
+    l ↦∗ ((g <$> xs) ++ replicate (n - i) #()) -∗
+    WP array_init_loop #l #i #n f @ stk; E {{ _, ∃ ys,
+       l ↦∗ (g <$> (xs ++ ys)) ∗ ⌜length (xs++ys) = n⌝ ∗ ([∗ list] k↦x∈(xs++ys), Q k x) }}.
+  Proof.
+    iIntros (Hn Hxs Hi) "Hxs #Hf Hl". iRevert (Hxs Hi).
+    iLöb as "IH" forall (xs i). iIntros (Hxs Hi).
+    wp_rec. wp_pures. case_bool_decide; simplify_eq/=; wp_pures.
+    - iExists []. iFrame.
+      assert (length xs - length xs = 0) as -> by lia.
+      rewrite !app_nil_r. eauto with iFrame.
+    - wp_bind (f #(length xs)). iApply (wp_wand with "Hf").
+      iIntros (v). iDestruct 1 as (x) "[-> Hx]".
+      wp_apply (wp_store_offset with "Hl").
+      { apply lookup_lt_is_Some_2.
+        rewrite app_length.
+        assert (length xs ≠ n) by naive_solver.
+        assert (n - length xs > 0) by lia.
+        rewrite fmap_length replicate_length. lia. }
+      iIntros "Hl". wp_pures.
+      assert ((Z.of_nat (length xs) + 1)%Z = Z.of_nat (length xs + 1)) as -> by lia.
+      iSpecialize ("IH" $! (xs++[x]) (length xs + 1) with "[Hx Hxs] [Hl] [%] [%]").
+      { rewrite big_sepL_app /= Nat.add_0_r. by iFrame. }
+      { assert (length xs = length xs + 0) as Hlen1 by lia.
+        rewrite {1}Hlen1.
+        rewrite -{1}(fmap_length g xs).
+        rewrite insert_app_r fmap_app /=.
+        rewrite app_assoc_reverse /=.
+        assert (length xs ≠ n) by naive_solver.
+        assert ((n - length xs) = S (n - (length xs + 1))) as -> by lia.
+        by rewrite insert_0_replicate. }
+      { by rewrite app_length. }
+      { assert (length xs ≠ n) by naive_solver. lia. }
+      iApply (wp_wand with "IH").
+      iIntros (_). iDestruct 1 as (ys) "(Hys & Hlen & HQs)".
+      iDestruct "Hlen" as %Hlen.
+      rewrite -app_assoc.
+      iExists ([x] ++ ys). iFrame. iPureIntro.
+      by rewrite app_assoc.
+  Qed.
+
+  Theorem wp_array_init {A : Type} (g : A → val) (Q : nat → A → iProp Σ)
+          n (f : val) stk E :
+    (0 < n)%Z →
+    {{{ (□ ∀ i : nat, WP f #i @ stk; E {{ v, ∃ x : A, ⌜v = g x⌝ ∗ Q i x }}) }}}
+      array_init #n f @ stk; E
+    {{{ l xs, RET #l; l ↦∗ (g<$>xs) ∗ ⌜Z.of_nat (length xs) = n⌝ ∗ ([∗ list] k↦x∈xs, Q k x) }}}.
+  Proof.
+    intros Hn. iIntros (Φ) "#Hf HΦ".
+    wp_rec. wp_pures. wp_alloc l as "Hl"; first done.
+    wp_pures.
+    iPoseProof (wp_array_init_loop g Q [] 0 (Z.to_nat n) with "[//] Hf [Hl]") as "H"; try by (simpl; lia).
+    { simpl. assert (Z.to_nat n - 0 = Z.to_nat n) as -> by lia. done. }
+    assert (Z.of_nat 0%nat = 0%Z) as -> by lia.
+    assert (Z.of_nat (Z.to_nat n) = n) as -> by lia.
+    wp_apply (wp_wand with "H").
+    iIntros (?). iDestruct 1 as (vs) "(Hl & % & HQs)".
+    wp_pures. iApply "HΦ".
+    iFrame "Hl HQs". iPureIntro. lia.
+  Qed.
+
+  Lemma wp_array_init' (Q : nat → val → iProp Σ) n (f : val) stk E :
+    (0 < n)%Z →
+    {{{ (□ ∀ i : nat, WP f #i @ stk; E {{ v, Q i v }}) }}}
+      array_init #n f @ stk; E
+    {{{ l xs, RET #l; l ↦∗ xs ∗ ⌜Z.of_nat (length xs) = n⌝ ∗ ([∗ list] k↦x∈xs, Q k x) }}}.
+  Proof.
+    intros Hn. iIntros (Φ) "#Hf HΦ".
+    iApply (wp_array_init id Q with "[Hf]"); try done.
+    { iModIntro. iIntros (i). iApply (wp_wand with "Hf").
+      iIntros (v) "Hv". iExists v; eauto with iFrame. }
+    iNext. iIntros (l xs). by rewrite list_fmap_id.
   Qed.
 
 End proof.
